Further Dfa proofs, a reference textbook, and a test

Cslib/Computability/Dfa/Basic.lean
@@ -6,10 +6,15 @@ Authors: Fabrizio Montesi
 
 import Cslib.Foundations.Semantics.Lts.Basic
 
+set_option linter.style.longLine false in
 /-! # Deterministic Finite-State Automata
 
 A Deterministic Finite-State Automaton (DFA) is a finite-state machine that accepts or rejects
 a finite string.
+
+## References
+
+* [J. E. Hopcroft, R. Motwani, J. D. Ullman, *Introduction to Automata Theory, Languages, and Computation*][Hopcroft2006]
 -/
 
 /-- A Deterministic Finite-State Automaton (DFA) consists of a labelled transition function
@@ -29,6 +34,38 @@ structure Dfa (State : Type _) (Symbol : Type _) where
 
 namespace Dfa
 
+/-- Extended transition function.
+
+Implementation note: compared to [Hopcroft2006], the definition consumes the input list of symbols
+from the left (instead of the right), in order to follow the way lists are constructed.
+-/
+@[grind]
+def mtr (dfa : Dfa State Symbol) (s : State) (xs : List Symbol) :=
+  match xs with
+  | [] => s
+  | x :: xs => dfa.mtr (dfa.tr s x) xs
+
+@[grind]
+theorem mtr_nil_eq {dfa : Dfa State Symbol} : dfa.mtr s [] = s := by rfl
+
+/-- A DFA accepts a trace if there is a multi-step accepting derivative with that trace from
+the start state. -/
+@[grind]
+def Accepts (dfa : Dfa State Symbol) (μs : List Symbol) :=
+  (dfa.mtr dfa.start μs) ∈ dfa.accept
+
+/-- The language of a DFA is the set of traces that it accepts. -/
+@[grind]
+def language (dfa : Dfa State Symbol) : Set (List Symbol) :=
+  { μs | dfa.Accepts μs }
+
+/-- A trace is accepted by a DFA iff it is in the language of the DFA. -/
+@[grind]
+theorem accepts_mem_language (dfa : Dfa State Symbol) (μs : List Symbol) :
+  dfa.Accepts μs ↔ μs ∈ dfa.language := by rfl
+
+section Lts
+
 /-- `Dfa` is a special case of `Lts`. -/
 @[grind]
 def toLts (dfa : Dfa State Symbol) : Lts State Symbol :=
@@ -37,10 +74,24 @@ def toLts (dfa : Dfa State Symbol) : Lts State Symbol :=
 instance : Coe (Dfa State Symbol) (Lts State Symbol) where
   coe := toLts
 
+/-- `Dfa.toLts` correctly characterises transitions. -/
 @[grind]
 theorem toLts_tr {dfa : Dfa State Symbol} :
   dfa.toLts.Tr s1 μ s2 ↔ dfa.tr s1 μ = s2 := by
   rfl
+
+/-- `Dfa.toLts` correctly characterises multistep transitions. -/
+@[grind]
+theorem toLts_mtr {dfa : Dfa State Symbol} :
+  dfa.toLts.MTr s1 xs s2 ↔ dfa.mtr s1 xs = s2 := by
+  constructor <;> intro h
+  case mp =>
+    induction h <;> grind
+  case mpr =>
+    induction xs generalizing s1
+    case nil => grind
+    case cons x xs ih =>
+      apply Lts.MTr.stepL (s2 := dfa.tr s1 x) <;> grind
 
 /-- The LTS induced by a DFA is deterministic. -/
 @[grind]
@@ -52,20 +103,6 @@ theorem toLts_deterministic (dfa : Dfa State Symbol) : dfa.toLts.Deterministic :
 theorem toLts_finiteState (dfa : Dfa State Symbol) : dfa.toLts.FiniteState :=
   dfa.finite_state
 
-/-- A DFA accepts a trace if there is a multi-step accepting derivative with that trace from
-the start state. -/
-@[grind]
-def Accepts (dfa : Dfa State Symbol) (μs : List Symbol) :=
-  ∃ s ∈ dfa.accept, dfa.toLts.MTr dfa.start μs s
-
-/-- The language of a DFA is the set of traces that it accepts. -/
-@[grind]
-def language (dfa : Dfa State Symbol) : Set (List Symbol) :=
-  { μs | dfa.Accepts μs }
-
-/-- A trace is accepted by a DFA iff it is in the language of the DFA. -/
-@[grind]
-theorem accepts_mem_language (dfa : Dfa State Symbol) (μs : List Symbol) :
-  dfa.Accepts μs ↔ μs ∈ dfa.language := by rfl
+end Lts
 
 end Dfa
