CslibTests/Dfa.lean
@@ -1,0 +1,48 @@
+/-
+Copyright (c) 2025 Fabrizio Montesi. All rights reserved.
+Released under Apache 2.0 license as described in the file LICENSE.
+Authors: Fabrizio Montesi
+-/
+
+import Cslib.Computability.Dfa.Basic
+
+/-! A simple elevator. -/
+
+inductive Floor where
+| one
+| two
+deriving DecidableEq
+
+def Floor.fintype : Fintype Floor := {
+  elems := {.one, .two}
+  complete floor := by grind [Floor]
+}
+
+theorem Floor.finite : Finite Floor := Floor.fintype.finite
+
+inductive Direction where
+| up
+| down
+deriving DecidableEq
+
+def Direction.fintype : Fintype Direction := {
+  elems := {.up, .down}
+  complete dir := by grind [Direction]
+}
+
+theorem Direction.finite : Finite Direction := Direction.fintype.finite
+
+def tr (floor : Floor) (dir : Direction) : Floor :=
+  match floor, dir with
+  | .one, .up => .two
+  | .one, .down => .one
+  | .two, .up => .two
+  | .two, .down => .one
+
+def elevator : Dfa Floor Direction := {
+  tr := tr
+  start := .one
+  accept := { Floor.one }
+  finite_state := Floor.finite
+  finite_symbol := Direction.finite
+}
